complete proofs of inset flow lemmas

inset_flows.v
@@ -1,3 +1,4 @@
+Require Import Coq.Numbers.NatInt.NZAddOrder.
 Set Default Proof Using "All".
 Require Export flows ccm.
 
@@ -6,7 +7,7 @@ Definition int_multiset := nzmap Z nat.
 
 Instance int_multiset_ccm : CCM int_multiset := lift_ccm Z nat.
 
-Definition dom_ms (m : int_multiset) := dom (gset Z) m.
+Definition dom_ms (m : int_multiset) := nzmap_dom Z nat m.
 
 Canonical Structure inset_flowint_ur : ucmraT := flowintUR int_multiset.
 
@@ -39,13 +40,128 @@ Definition globalinv root I : Prop := ✓I ∧ (root ∈ domm I) ∧ (∀ k n, k
                                              ∧ ((n ≠ root) → (∀ k, k ∉ inset I n)).  
 
 Lemma flowint_step :
-  ∀ I I1 I2 k n root, I = I1 ⋅ I2 → ✓I → k ∈ outset I1 n → globalinv root I → n ∈ domm I2.
+  ∀ I I1 I2 k n root, globalinv root I → I = I1 ⋅ I2 → k ∈ outset I1 n → n ∈ domm I2.
 Proof.
-  intros.
-  unfold globalinv in H2.
-  destruct H2.
-  destruct H3.
-  destruct H4.
-  (*assert (n inf I n = out I1 n + out I2 n)*)
-  (* TODO: lemma_int_comp_unfold *)
-Admitted.
+  intros I I1 I2 k n r gInv dI kOut.
+  unfold globalinv in gInv.
+  destruct gInv as [vI [rI [cI H]]].
+  
+  assert (domm I = domm I1 ∪ domm I2) as disj.
+  eauto using intComp_dom.
+
+  assert (✓ I1) as vI1.
+  rewrite dI in vI.
+  eauto using intComp_valid_proj1.
+
+  apply flowint_valid_unfold in vI1.
+  destruct vI1 as [Ir1 [dI1 [disj1 _]]].
+
+  (* First, prove n ∉ domm I1 *)
+  
+  assert (is_Some (out I1 n !! k)) as out1nk.
+  unfold outset, dom_ms, nzmap_dom in kOut.
+  by rewrite nzmap_elem_of_dom in kOut *.
+
+  assert (is_Some (outR Ir1 !! n)) as out1n.
+  unfold out, out_map in out1nk.
+  rewrite dI1 in out1nk.
+  destruct (outR Ir1 !! n).
+  eauto.
+  lazy in out1nk.
+  destruct out1nk.
+  Transparent gmap_empty.
+  unfold gmap_empty in H0.
+  unfold empty in H0.
+  simpl in H0.
+  inversion H0.
+
+  assert (n ∈ dom (gset Node) (outR Ir1)) as inOut1n.
+  by apply elem_of_dom.
+
+  assert (dom (gset Node) (infR Ir1) ## dom (gset Node) (outR Ir1)) as domDisj1.
+  by apply map_disjoint_dom.
+
+  assert (n ∉ dom (gset Node) (infR Ir1)) as not_in_Inf1_n.
+  set_solver.
+
+  (* Now, prove n ∈ domm I *)
+
+  assert (vI' := vI).
+  apply flowint_valid_unfold in vI'.
+  destruct vI' as [Ir [dI' [disj' _]]].
+
+  assert (n ∈ dom (gset Node) (infR Ir)) as in_Inf_n.
+  rewrite dI in vI.
+  pose proof (intComp_unfold_out I1 I2 vI n).
+  destruct (decide (n ∉ domm (I1 ⋅ I2))).
+  apply H0 in n0.
+  pose proof (cI k n) as not_k_out.
+  unfold outset, dom_ms, nzmap_dom in not_k_out.
+  apply not_elem_of_dom in not_k_out.
+  assert (out I n !! k = out (I1 ⋅ I2) n !! k).
+  rewrite dI. reflexivity.
+  rewrite n0 in H1.
+  unfold ccmop, ccm_op in H1.
+  unfold int_multiset_ccm in H1.
+  unfold lift_ccm in H1.
+  unfold lift_op in H1.
+  case_eq (out I1 n).
+  intros ? ? out1.
+  rewrite out1 in H1.
+  case_eq (out I2 n).
+  intros ? ? out2.
+  rewrite out2 in H1.
+  unfold lookup at 2 in H1.
+  unfold nzmap_lookup in H1.
+  rewrite lookup_merge in H1.
+  unfold merge_op in H1.
+  assert (out I1 n !! k = nzmap_car !! k).
+  rewrite out1. unfold lookup at 1. by unfold nzmap_lookup.
+  rewrite <- H2 in H1.
+  unfold is_Some in out1nk.
+  destruct out1nk as [x1 out1nk].
+  rewrite out1nk in H1.
+  assert (x1 <> 0) as x1_pos.
+  pose proof (nzmap_is_wf _ _ (out I1 n)).
+  rewrite out1 in H3. simpl in H3.
+  pose proof (nzmap_lookup_wf _ _ _ k H3).
+  rewrite <- H2 in H4.
+  rewrite out1nk in H4.
+  clear - H4.
+  firstorder.
+
+  destruct (nzmap_car0 !! k);
+  try destruct decide in H1;
+  first [
+         clear - e x1_pos;
+         (* TODO: There must be a better way of doing this... *)
+         unfold ccm_unit, ccmunit, nat_ccm, nat_unit, ccm_op, ccmop, nat_op in e; simpl;
+         lia |
+         unfold ccm.nzmap_car in not_k_out;
+           unfold lookup in H1;
+           case_eq (out I n);
+           intros;
+           rewrite H3 in H1;
+           rewrite H3 in not_k_out;
+           unfold lookup in not_k_out;
+           rewrite not_k_out in H1;
+           inversion H1].
+
+  unfold domm, dom, flowint_dom, inf_map in n0.
+  rewrite <- dI in n0.
+  rewrite dI' in n0.
+  apply dec_stable in n0.
+  trivial.
+  
+  (* Finally, prove n ∈ domm I2 *)
+  
+  unfold domm, dom, flowint_dom.
+  unfold domm, dom, flowint_dom in disj.
+  unfold inf_map at 1 in disj; rewrite dI' in disj.
+  unfold inf_map at 1 in disj; rewrite dI1 in disj.
+  rewrite elem_of_equiv_L in disj *.
+  intro dom_I.
+  pose proof (dom_I n) as dom_I_n.
+  rewrite elem_of_union in dom_I_n *.
+  naive_solver.
+Qed.
